transition to mandatory structure

theories/BinaryStackMachines/BSM/bsm_defs.v
@@ -14,6 +14,9 @@ From Undecidability.Shared.Libs.DLW
                  Vec.pos Vec.vec
                  Code.subcode Code.sss.
 
+From Undecidability.BinaryStackMachines 
+  Require Export BSM.
+
 Set Implicit Arguments.
 
 Tactic Notation "rew" "length" := autorewrite with length_db.
@@ -21,40 +24,13 @@ Tactic Notation "rew" "length" := autorewrite with length_db.
 Local Notation "e #> x" := (vec_pos e x).
 Local Notation "e [ v / x ]" := (vec_change e x v).
 
-(** * Binary Stack Machines
-   Binary stack machines have n stacks and there are just two instructions
-  
-   1/ POP s p q : pops the value on stack s and
-                  if Empty then jumps to q 
-                  if Zero then jumps to p
-                  if One then jumps to next instruction,
-   2/ PUSH s b : pushes the value b on stack s and jumps to next instructions 
-
- *)
-
-Inductive bsm_instr n : Set :=
-  | bsm_pop  : pos n -> nat -> nat -> bsm_instr n
-  | bsm_push : pos n -> bool -> bsm_instr n
-  .
-
-Notation POP  := bsm_pop.
-Notation PUSH := bsm_push.
-
-
-(** ** Semantics for BSM *)
+(** ** Semantics results for BSM *)
 
 Section Binary_Stack_Machine.
 
   Variable (n : nat).
 
-  Definition bsm_state := (nat*vec (list bool) n)%type.
-
-  Inductive bsm_sss : bsm_instr n -> bsm_state -> bsm_state -> Prop :=
-    | in_bsm_sss_pop_E : forall i x p q v,    v#>x = nil      -> POP x p q // (i,v) -1> (  q,v)
-    | in_bsm_sss_pop_0 : forall i x p q v ll, v#>x = Zero::ll -> POP x p q // (i,v) -1> (  p,v[ll/x])
-    | in_bsm_sss_pop_1 : forall i x p q v ll, v#>x = One ::ll -> POP x p q // (i,v) -1> (1+i,v[ll/x])
-    | in_bsm_sss_push  : forall i x b v,                         PUSH x b  // (i,v) -1> (1+i,v[(b::v#>x)/x])
-  where "i // s -1> t" := (bsm_sss i s t).
+  Notation "i // s -1> t" := (@bsm_sss n i s t).
 
   Ltac mydiscr := 
       match goal with H: ?x = _, G : ?x = _ |- _ => rewrite H in G; discriminate end.
@@ -90,7 +66,7 @@ Section Binary_Stack_Machine.
      that the state cannot change anymore (this is a strictly lesser requirement).
   *)
   
-  Fact bsm_sss_stall : forall P s, sss_step_stall bsm_sss P s -> out_code (fst s) P.
+  Fact bsm_sss_stall : forall P s, sss_step_stall (@bsm_sss n) P s -> out_code (fst s) P.
   Proof.
     intros (i,P) (q,v) H; unfold fst.
     red in H.
@@ -102,8 +78,8 @@ Section Binary_Stack_Machine.
     apply (H t); subst; apply in_sss_step; auto.
   Qed.
  
-  Notation "P // s -[ k ]-> t" := (sss_steps bsm_sss P k s t).
-  Notation "P // s ->> t" := (sss_compute bsm_sss P s t).
+  Notation "P // s -[ k ]-> t" := (sss_steps (@bsm_sss n) P k s t).
+  Notation "P // s ->> t" := (sss_compute (@bsm_sss n) P s t).
 
   Fact bsm_compute_POP_E P i x p q v st :
          (i,POP x p q::nil) <sc P
@@ -296,15 +272,3 @@ Tactic Notation "bsm" "inv" "PUSH" "with" hyp(H) constr(a) constr(c) :=
      apply bsm_steps_PUSH_inv with (x := a) (b := c) in H; auto.
 
 Hint Immediate bsm_sss_fun : core.
-
-(* The Halting problem for BSM *)
-  
-Definition BSM_PROBLEM := { n : nat & { i : nat & { P : list (bsm_instr n) & vec (list bool) n } } }.
-
-Local Notation "P // s ↓" := (sss_terminates (@bsm_sss _) P s).
-
-Definition BSM_HALTING (P : BSM_PROBLEM) := 
-  match P with existT _ n (existT _ i (existT _ P v)) => (i,P) // (i,v) ↓ end.
-
-
-     
