theories/BinaryStackMachines/BSM_undec.v
@@ -1,0 +1,27 @@
+(**************************************************************)
+(*   Copyright Dominique Larchey-Wendling [*]                 *)
+(*                                                            *)
+(*                             [*] Affiliation LORIA -- CNRS  *)
+(**************************************************************)
+(*      This file is distributed under the terms of the       *)
+(*         CeCILL v2 FREE SOFTWARE LICENSE AGREEMENT          *)
+(**************************************************************)
+
+Require Import List Bool.
+
+From Undecidability.Shared.Libs.DLW 
+  Require Import Utils.list_bool Vec.pos Vec.vec Code.sss.
+
+From Undecidability.BinaryStackMachines 
+  Require Import BSM Reductions.iBPCP_BSM.
+
+Require Import Undecidability.Synthetic.Undecidability.
+
+From Undecidability.PCP
+  Require Import PCP PCP_undec.
+
+Theorem BSM_undec : undecidable (BSM_HALTING).
+Proof.
+  apply (undecidability_from_reducibility iPCPb_undec).
+  apply iBPCP_BSM_HALTING.
+Qed.
