theories/ILL/Reductions/HALT_MM.v
@@ -16,23 +16,19 @@ From Undecidability.Shared.Libs.DLW.Vec Require Import pos vec.
 From Undecidability.Shared.Libs.DLW.Utils Require Import utils_tac.
 From Undecidability.MinskyMachines Require Import mm_defs.
 
-From Undecidability.ILL Require Import UNDEC.
+(* From Undecidability.ILL Require Import UNDEC. *)
 
-From Undecidability.StringRewriting Require Import Util.singleTM Reductions.TM_to_SRH Reductions.SRH_to_SR.
-From Undecidability.PCP Require Import Reductions.SR_to_MPCP Reductions.MPCP_to_PCP.
+Require Import Undecidability.Synthetic.Undecidability.
+Require Import Undecidability.TM.Halting.
+Require Import Undecidability.PCP.Reductions.HALT_TM1_to_PCPb.
 
 Set Implicit Arguments.
 
-Corollary Halt_PCP : Halt ⪯ PCP.
-Proof.
-  eapply reduces_transitive. exact TM_to_SRH.Halt_SRH.
-  eapply reduces_transitive. exact SRH_to_SR.reduction.
-  eapply reduces_transitive. exact SR_to_MPCP.reduction.
-  exact MPCP_to_PCP.reduction.
-Qed.
+Lemma BSM_MM_HALT
 
-Corollary MM_HALTING_undec : Halt ⪯ MM_HALTING.
+Corollary MM_HALTING_undec : undecidable MM_HALTING.
 Proof.
+  apply (undecidability_from_reducibility BSM_undec).
   eapply reduces_transitive. exact Halt_PCP.
   exact PCP_MM_HALTING.
 Qed.
