theories/PCP/Reductions/HALT_TM1_to_PCPb.v
@@ -1,0 +1,38 @@
+(**************************************************************)
+(*   Copyright Dominique Larchey-Wendling [*]                 *)
+(*                                                            *)
+(*                             [*] Affiliation LORIA -- CNRS  *)
+(**************************************************************)
+(*      This file is distributed under the terms of the       *)
+(*         CeCILL v2 FREE SOFTWARE LICENSE AGREEMENT          *)
+(**************************************************************)
+
+(* Direct reductions from Halting of 1-TM to binary PCP *)
+
+Require Import Undecidability.Synthetic.Undecidability.
+
+Require Import Undecidability.TM.Halting.
+
+From Undecidability.StringRewriting.Reductions
+  Require Import TM_to_SRH SRH_to_SR.
+
+From Undecidability.PCP
+  Require Import PCP.
+
+From Undecidability.PCP.Reductions
+  Require Import SR_to_MPCP MPCP_to_PCP PCP_to_PCPb.
+
+Lemma HALT_TM1_to_PCP : HaltTM 1 ⪯ PCP.
+Proof.
+  eapply reduces_transitive. exact singleTM.TM_conv.
+  eapply reduces_transitive. exact Halt_SRH.
+  eapply reduces_transitive. exact SRH_to_SR.reduction.
+  eapply reduces_transitive. exact SR_to_MPCP.reduction.
+  exact MPCP_to_PCP.reduction.
+Qed.
+
+Lemma HALT_TM1_to_PCPb : HaltTM 1 ⪯ PCPb.
+Proof.
+  eapply reduces_transitive. exact HALT_TM1_to_PCP.
+  exact PCP_to_PCPb.reduction.
+Qed.
